pcuic/theories/PCUICUnivSubst.v
@@ -6,7 +6,8 @@ Lemma lift_subst_instance_constr u c n k :
   lift n k (subst_instance_constr u c) = subst_instance_constr u (lift n k c).
 Proof.
   induction c in k |- * using term_forall_list_ind; simpl; auto;
-    rewrite ?map_map_compose, ?compose_on_snd, ?compose_map_def, ?map_length;
+    rewrite ?map_map_compose, ?compose_on_snd, ?compose_map_def, ?map_length,
+      ?map_predicate_map_predicate, ?map_branch_map_branch;
     try solve [f_equal; eauto; solve_all; eauto].
 Qed.
 
@@ -36,7 +37,8 @@ Lemma subst_subst_instance_constr u c N k :
   = subst_instance_constr u (subst N k c).
 Proof.
   induction c in k |- * using term_forall_list_ind; simpl; auto;
-    rewrite ?map_map_compose, ?compose_on_snd, ?compose_map_def, ?map_length;
+    rewrite ?map_map_compose, ?compose_on_snd, ?compose_map_def, ?map_length,
+      ?map_branch_map_branch, ?map_predicate_map_predicate;
     try solve [f_equal; eauto; solve_all; eauto].
 
   elim (Nat.leb k n). rewrite nth_error_map.
@@ -52,44 +54,23 @@ Proof.
   solve_all. now destruct H as [n [-> _]].
 Qed.
 
-(** Tests that the term is closed over [k] universe variables *)
-Fixpoint closedu (k : nat) (t : term) : bool :=
-  match t with
-  | tSort univ => closedu_universe k univ
-  | tInd _ u => closedu_instance k u
-  | tConstruct _ _ u => closedu_instance k u
-  | tConst _ u => closedu_instance k u
-  | tRel i => true
-  | tEvar ev args => forallb (closedu k) args
-  | tLambda _ T M | tProd _ T M => closedu k T && closedu k M
-  | tApp u v => closedu k u && closedu k v
-  | tLetIn na b t b' => closedu k b && closedu k t && closedu k b'
-  | tCase ind p c brs =>
-    let brs' := forallb (test_snd (closedu k)) brs in
-    closedu k p && closedu k c && brs'
-  | tProj p c => closedu k c
-  | tFix mfix idx =>
-    forallb (test_def (closedu k) (closedu k)) mfix
-  | tCoFix mfix idx =>
-    forallb (test_def (closedu k) (closedu k)) mfix
-  | x => true
-  end.
-
 Lemma closedu_subst_instance_constr u t
   : closedu 0 t -> subst_instance_constr u t = t.
 Proof.
   induction t in |- * using term_forall_list_ind; simpl; auto; intros H';
-    rewrite -> ?map_map_compose, ?compose_on_snd, ?compose_map_def, ?map_length;
-    try f_equal; eauto with substu; unfold test_def in *;
-      try solve [f_equal; eauto; repeat (rtoProp; solve_all)].
+    rewrite -> ?map_map_compose, ?compose_on_snd, ?compose_map_def, ?map_length,
+      ?map_branch_map_branch, ?map_predicate_map_predicate;
+    try f_equal; eauto with substu; unfold test_predicate, test_def in *;
+      try solve [f_equal; eauto; repeat (rtoProp; solve_all); eauto with substu].
 Qed.
 
 Lemma subst_instance_constr_closedu (u : Instance.t) (Hcl : closedu_instance 0 u) t :
   closedu #|u| t -> closedu 0 (subst_instance_constr u t).
 Proof.
   induction t in |- * using term_forall_list_ind; simpl; auto; intros H';
-    rewrite -> ?map_map_compose, ?compose_on_snd, ?compose_map_def, ?map_length, ?forallb_map;
+    rewrite -> ?map_map_compose, ?compose_on_snd, ?compose_map_def, ?map_length, ?forallb_map,
+      ?map_predicate_map_predicate;
     try f_equal; auto with substu;
-      unfold test_def, map_def in *;
-      try solve [f_equal; eauto; repeat (rtoProp; solve_all); intuition auto with substu].
+      unfold test_def, test_predicate in *; simpl;
+      f_equal; eauto; repeat (rtoProp; solve_all); intuition auto with substu.
 Qed.
